src/proof/controllers/statefulset/create_pvc.v
@@ -1,0 +1,128 @@
+From New.proof Require Import prelude empty_ffi.
+From New.proof.controllers.statefulset Require Export pvc.
+
+Section proof.
+Context `{hG: !heapGS Σ} `{!ffi_semantics _ _}.
+Context {sem : go.Semantics}
+  {package_sem : code.controllers.statefulset.statefulset.Assumptions}.
+Collection W := sem + package_sem.
+#[local] Instance base_common_sem : common.Assumptions | 100 :=
+  code.controllers.statefulset.statefulset.import_common_Assumption.
+#[local] Instance controller_sem : controller.Assumptions :=
+  code.controllers.statefulset.statefulset.import_controller_Assumption.
+#[local] Instance runtime_sem :
+    code.k8s_io.apimachinery.pkg.runtime.runtime.Assumptions :=
+  controller.import_runtime_Assumption.
+#[local] Instance runtime_object_underlying_eq :
+    runtime.Object ≤u runtime.Objectⁱᵐᵖˡ.
+Proof using package_sem. apply _. Qed.
+#[local] Instance meta_object_underlying_eq :
+    meta_v1.Object ≤u meta_v1.Objectⁱᵐᵖˡ.
+Proof using package_sem. apply _. Qed.
+#[local] Instance base_apimodel_sem : apimodel.Assumptions | 100 :=
+  common.import_apimodel_Assumption.
+#[local] Instance object_meta_v1_sem :
+    code.k8s_io.apimachinery.pkg.apis.meta.v1.v1.Assumptions :=
+  apimodel.import_apis_meta_v1_Assumption.
+#[local] Instance object_apps_v1_sem :
+    code.k8s_io.api.apps.v1.v1.Assumptions :=
+  apimodel.import_api_apps_v1_Assumption.
+#[local] Instance object_core_v1_sem :
+    code.k8s_io.api.core.v1.v1.Assumptions :=
+  code.k8s_io.api.apps.v1.v1.import_core_v1_Assumption.
+#[local] Instance apimodel_sem : apimodel.Assumptions | 0.
+Proof using package_sem.
+  constructor; try exact object_core_v1_sem; try apply _.
+Defined.
+#[local] Instance common_sem : common.Assumptions | 0.
+Proof using package_sem.
+  constructor; try exact apimodel_sem; try apply _.
+Defined.
+Context `{!kubernetesModelG Σ}.
+Local Set Default Proof Using "All".
+
+Definition new_persistent_volume_claim_key
+    (set : StatefulSetV.t) (claim_template : PersistentVolumeClaimV.t)
+    (ordinal : nat) : KKey.t :=
+  PersistentVolumeClaimV.key
+    (new_persistent_volume_claim set claim_template ordinal).
+
+(* The controller only needs metadata and spec fragments to remember that the
+   PVC exists.  The model's metadata-fragment validity ties the UID used by
+   both fragments to the PVC metadata. *)
+Definition persistent_volume_claim_exists γ key : iProp Σ :=
+  ∃ claim,
+    "%Hkey" ∷ ⌜ PersistentVolumeClaimV.key claim = key ⌝ ∗
+    "Hmeta" ∷ own_meta_frag γ key
+      claim.(PersistentVolumeClaimV.ObjectMeta').(ObjectMetaV.UID') 1
+      claim.(PersistentVolumeClaimV.ObjectMeta') ∗
+    "Hspec" ∷ own_spec_frag γ key
+      claim.(PersistentVolumeClaimV.ObjectMeta').(ObjectMetaV.UID') 1
+      (ObjectSpecV.PersistentVolumeClaimSpec
+        claim.(PersistentVolumeClaimV.Spec')).
+
+(* [createPersistentVolumeClaim] is an idempotent ensure operation.  If the
+   claim already exists, Get succeeds and its fragments are preserved.  If its
+   key is reserved, the Kubernetes model guarantees that it is absent, so the
+   NotFound branch creates it and consumes the reservation. *)
+Lemma wp_createPersistentVolumeClaim γ model_l
+    set_l pod_l claim_template_l
+    (set : StatefulSetV.t) (pod : PodV.t)
+    (claim_template : PersistentVolumeClaimV.t) (ordinal : nat)
+    dq_set dq_pod dq_claim_template :
+  {{{ "#Hpkg" ∷
+        is_pkg_init code.controllers.statefulset.pkg_id.statefulset ∗
+      "#Hisk" ∷ is_kubernetes γ model_l ∗
+      "#Hglobal_l" ∷
+        (global_addr apimodel.ModelState) ↦□ model_l ∗
+      "Hset" ∷ StatefulSetV.deepown_l set_l set dq_set ∗
+      "Hpod" ∷ PodV.deepown_l pod_l pod dq_pod ∗
+      "Hclaim_template" ∷
+        PersistentVolumeClaimV.deepown_l
+          claim_template_l claim_template dq_claim_template ∗
+      "%Hordinal_bound" ∷
+        ⌜ (ordinal ≤ go_int32_max_nat)%nat ⌝ ∗
+      "%Hpod_name" ∷
+        ⌜ pod.(PodV.ObjectMeta').(ObjectMetaV.Name') =
+            desired_pod_name
+              set.(StatefulSetV.ObjectMeta').(ObjectMetaV.Name')
+              ordinal ⌝ ∗
+      "%Hpod_name_len" ∷
+        ⌜ Z.of_nat
+            (length pod.(PodV.ObjectMeta').(ObjectMetaV.Name')) ≤
+          go_int_max ⌝ ∗
+      "Hpvc_state" ∷
+        (persistent_volume_claim_exists γ
+            (new_persistent_volume_claim_key
+              set claim_template ordinal) ∨
+         ("Hreserved" ∷ own_reserved_frag γ
+            (new_persistent_volume_claim_key
+              set claim_template ordinal) ∗
+          "%Hvalid_create" ∷
+            ⌜ PersistentVolumeClaimV.valid_named_create
+                set.(StatefulSetV.ObjectMeta').(ObjectMetaV.Namespace')
+                (new_persistent_volume_claim
+                  set claim_template ordinal) ⌝ ∗
+          "%Hnamespace_nonempty" ∷
+            ⌜ set.(StatefulSetV.ObjectMeta').(ObjectMetaV.Namespace') ≠
+                ""%go ⌝ ∗
+          "%Hnamespace_valid" ∷
+            ⌜ valid_namespace
+                set.(StatefulSetV.ObjectMeta').(ObjectMetaV.Namespace') ⌝))
+  }}}
+    @! statefulset.createPersistentVolumeClaim
+      #set_l #pod_l #claim_template_l
+  {{{ RET #interface.nil;
+      "Hset" ∷ StatefulSetV.deepown_l set_l set dq_set ∗
+      "Hpod" ∷ PodV.deepown_l pod_l pod dq_pod ∗
+      "Hclaim_template" ∷
+        PersistentVolumeClaimV.deepown_l
+          claim_template_l claim_template dq_claim_template ∗
+      "Hpvc_state" ∷
+        persistent_volume_claim_exists γ
+          (new_persistent_volume_claim_key
+            set claim_template ordinal)
+  }}}.
+Proof. Admitted.
+
+End proof.
